bir_typing_expTheory now updated with revised extern handling

src/theory/bir/bir_envScript.sml
@@ -353,12 +353,26 @@ val bir_envty_includes_vs_SUBSET = store_thm("bir_envty_includes_vs_SUBSET", ``
 
 val _ = Datatype `bir_var_ext_env_typing_t = BExtEnvTy (string -> (bir_type_t option))`;
 
+val bir_ext_envty_of_ext_env_def = Define `bir_ext_envty_of_ext_env ((BExtMap ext_get_map ext_put_map):'ext_state_t bir_ext_map_t, ext_st) =
+  BExtEnvTy (( \ f. OPTION_BIND f ( \ f'. OPTION_MAP type_of_bir_val (f' ext_st))) o (FLOOKUP ext_get_map))
+`;
+
+(* Note that this is only defined for get functions, for now... *)
 val bir_ext_env_satisfies_ext_envty_def = Define `
   bir_ext_env_satisfies_ext_envty (ext_map, ext_st:'ext_state_t) (BExtEnvTy ext_envty) <=>
     !ext_name ty.
       ext_envty ext_name = SOME ty ==>
       ?f_get v. bir_lookup_get ext_map ext_name = SOME f_get /\
           f_get ext_st = SOME v /\ type_of_bir_val v = ty`;
+
+val bir_ext_env_satisfies_ext_envty_of_ext_env = store_thm("bir_ext_env_satisfies_ext_envty_of_ext_env", ``
+  !ext_map (ext_st:'ext_state_t). bir_ext_env_satisfies_ext_envty (ext_map, ext_st) (bir_ext_envty_of_ext_env (ext_map, ext_st))
+``,
+  Cases_on `ext_map` >>
+  SIMP_TAC std_ss [bir_ext_env_satisfies_ext_envty_def, bir_ext_envty_of_ext_env_def, bir_lookup_get_def] >>
+  rpt strip_tac >>
+  metis_tac[]
+);
 
 val bir_ext_envty_includes_ext_def = Define `
   bir_ext_envty_includes_ext (BExtEnvTy ext_envty) (ext_name, ext_ty) <=>
@@ -379,6 +393,21 @@ val bir_eval_extget_def = Define `
         else SOME v
        | NONE => NONE)
     | NONE => NONE)`;
+
+val bir_eval_extget_type = store_thm ("bir_eval_extget_type",
+``!ext_map (ext_st:'ext_state_t) ext_name ext_ty v.
+  bir_eval_extget ext_map ext_name ext_ty ext_st = SOME v ==>
+  type_of_bir_val v = ext_ty``,
+
+  rpt strip_tac >>
+  fs[bir_eval_extget_def] >>
+  Cases_on `bir_lookup_get ext_map ext_name` >> (
+    fs[]
+  ) >>
+  Cases_on `x ext_st` >> (
+    gvs[]
+  )
+);
 
 val bir_ext_in_ext_envty_ext_env_IMP = store_thm ("bir_ext_in_ext_envty_ext_env_IMP",
 ``!ext_envty ext_map (ext_st:'ext_state_t) ext_name ext_ty.
